\subsection{Ring Homomorphisms}
\begin{definition}
	Given two rings $R,S,$ a function $\phi: R \to S$ is a ring homomorphism if
	\begin{enumerate}[label=\roman*)]
		\item $\phi(a+b) = \phi(a) + \phi(b)$ 
		\item $\phi(ab) = \phi(a)\phi(b)$
		\item $\phi(1_R) = 1_{S}$
	\end{enumerate}
\end{definition}
Notice that, by this definition, we're specifically examining the homomorphism on both operations. The definition of the kernel and image remains invariant under this definition. Furthermore, the property relating to injectivity by way of the kernel criterion remains the same as well.
\begin{proposition}
	Let $\phi : R \to S$ be a ring homomorphism. Then $\ker(\phi)$ is an ideal of $R$.
\end{proposition}
\begin{proof}
	Let $a \in \ker(\phi)$ and $r \in R$. Then 
	\begin{equation*}
		\phi(ar) = \phi(a)\phi(r) = 0\phi(r) = 0, \quad \phi(ra) = \phi(r)\phi(a) = \phi(r)0 = 0
	\end{equation*}
	so $ar,ra \in \ker(\phi)$. Since $\ker(\phi)$ is a subring, it must be true that $\ker(\phi)$ is closed under addition. Thus, $\ker(\phi)$ is an ideal.
\end{proof}
Naturally with this in mind, if we prove that $\phi$ is also a surjection, then we have a \textit{ring isomorphism}.

\subsection{The Canonical Projection}
\begin{theorem}
	Let $R$ be a ring and $I \unlhd R$ be an ideal. Then define the canonical projection
	\begin{equation*}
		\pi:R \to R/I, \quad \pi(r) = r+I
	\end{equation*}
	Then 
	\begin{enumerate}[label=(\roman*)]
		\item $\pi$ is a homomorphism
		\item $\pi$ is surjective
		\item $\ker(\pi) = I$
	\end{enumerate}
\end{theorem}
The canonical projection is what allows us to go from the ring $R$ to the quotient ring $R/I$. Notice though that this map is not injective, as certain elements may exist within the same equivalence class.

\begin{proof}
	Let $r,s \in R$. 
	\begin{enumerate}
		\item Additivity:
		\begin{equation*}
			\pi(r+s) = (r+s) + I = (r+I)+(s+I) = \pi(r) + \pi(s)
		\end{equation*}
		\item Multiplicativity:
		\begin{equation*}
			\pi(rs) = (rs+I) = (r+I)(s+I) = \pi(r)\pi(s)
		\end{equation*}
		\item Identity: 
		\begin{equation*}
			\pi(1) = 1+I
		\end{equation*}
	\end{enumerate}
	Thus, $\pi$ is a homomorphism. Surjectivity is trivial in how we define the map. Now consider the kernel. By definition
	\begin{equation*}
		\ker(\phi) = \set{r \in R: \pi(r) = 0+I} = \set{r \in R: r \in I} = I 
	\end{equation*}
\end{proof}

\subsection{Isomorphism Theorems}
\begin{theorem}[Mapping Property]
	Let $R,S$ be rings and let 
	\begin{equation*}
		\phi: R\to S
	\end{equation*}
	be a ring homomorphism. If $I \subseteq \ker(\phi)$, then there exists a unique ring homomorphism
	\begin{equation*}
		\overline{\phi}: R/I \to S
	\end{equation*}
	such that $\phi = \overline{\phi} \circ \pi $ where $\pi: R \to R/I$ is the canonical projection map. 
\end{theorem}

Not every homomorphism sends elements of an ideal to $0$. The mapping property requires $I \subseteq \ker\phi$; only then does the quotient $R/I$ allow a well-defined factorization. Otherwise, cosets could map ambiguously.
\begin{figure}[h!]
	\begin{center}
		\includegraphics[scale=.3]{MAPPINGPROPERTY}
		\caption{Diagram of the mapping property in action}
	\end{center}
\end{figure}
\begin{proof}
	First, define the map 
	\begin{equation*}
		\overline{\phi} (r+I) = \phi(r)
	\end{equation*}
	Now suppose $r+I=r'+I$. Then 
	\begin{equation*}
		r-r' \in I \subseteq \ker(\phi)
	\end{equation*}
	so 
	\begin{equation*}
		\phi(r-r') = 0 \imp \phi(r)=\phi(r')
	\end{equation*}
	Hence, $\overline{\phi}$ is well defined. Now, let us confirm that the map is in fact a homomorphism. Let $r,s \in R$.
	\begin{enumerate}
		\item Additivity:
		\begin{equation*}
			\overline{\phi}((r+I)+(s+I)) = \overline{\phi}(r+s+I) = \phi(r+s) = \phi(r) + \phi(s) = \overline{\phi}(r+I)+\overline{\phi}(s+I)
		\end{equation*}
		\item Multiplicity: 
		\begin{equation*}
			\overline{\phi}((r+I)(s+I)) = \overline{\phi}(rs+I) = \phi(r)\phi(s) = \overline{\phi}(r+I)\overline{\phi}(s+I)
		\end{equation*}
		\item Identity:
		\begin{equation*}
			\overline{\phi}(1+I) = \phi(1) = 1
		\end{equation*}
	\end{enumerate}
	Thus, $\overline{\phi}$ is a ring homomorphism. So notice then that 
	\begin{equation*}
		(\overline{\phi}\circ \pi)(r) = \overline{\phi}(r+I) = \phi(r)
	\end{equation*}
	so $\phi = \overline{\phi}\circ \pi$. Now, suppose $\psi:R/I \to S$ is any ring homomorphism with $\phi = \psi \circ \pi$. Then for any $r+I \in R/I$,
	\begin{equation*}
		\psi(r+I) = \psi(\pi(r)) = \phi(r) = \overline{\phi}(r+I)
	\end{equation*}
	Thus, $\psi = \overline{\phi}$, proving uniqueness.
\end{proof}
\begin{corollary}[First Isomorphism Theorem]
	Let $\phi: R\to S$ be a ring homomorphism. Then 
	\begin{equation*}
		R/\ker(\phi) \cong \text{im}\phi
	\end{equation*}
\end{corollary}
The use of the kernel as the ideal to quotient by is key for inducing injectivity, as all elements that map to 0 are collapsed to a singular representation.

\begin{theorem}[Second Isomorphism Theorem]
	Let $R$ be a ring, let $S\subseteq R$ be a subring, and let $I \unlhd R$ be an ideal. Then
	\begin{enumerate}[label=(\roman*)]
		\item $S\cap I \unlhd S$
		\item $S+I = \set{s+i: s \in S, i \in I}$ is a subring of $R$
		\item There is a natural ring isomorphism
		\begin{equation*}
			(S+I)/I \cong S/(S\cap I)
		\end{equation*}
	\end{enumerate}
\end{theorem}

\begin{theorem}[Third Isomorphism Theorem]
	Let $R$ be a ring and $I,K \unlhd R$ be ideals. Then
	\begin{equation*}
		(R/K)/(I/K) \cong R/I
	\end{equation*}
\end{theorem}

\subsection{Correspondence Theorem}
\begin{theorem}
	Let $R$ be a ring and let $I \unlhd R$ be an ideal. Then there is a one to one correspondence between
	\begin{enumerate}
		\item Ideals of $R$ containing $I$
		\item Ideals of the quotient ring $R/I$
	\end{enumerate}
	The correspondence is given by 
	\begin{equation*}
		J \mt J/I = \set{j+I: j \in J}, \quad \overline{J} \mt \pi^{-1}(\overline{J}) = \set{r \in R: r+I \in J}
	\end{equation*}
\end{theorem}
\begin{proof}
	Let $R$ be a ring and $I \unlhd R$ be an ideal. Then let $J$ be an ideal of $R$ such that $I \subseteq J$. Define a map
	\begin{equation*}
		\psi(r) = r+I
	\end{equation*}
	Return to $J$. Under the map $\psi$, we have that $J$ becomes
	\begin{equation*}
		J/I = \set{j+I: j \in J}
	\end{equation*}
	We'll now show that this resulting set is an ideal of $R/I$. Let $r+I \in R/I$ and $j+I \in J$. Then we have that
	\begin{equation*}
		(r+I)(j+I) = (rj+I)
	\end{equation*}
	Because $J$ was an ideal, we have that $rj \in J$. Thus, it must be true that $rj+I \in J/I$. Therfore, $J/I$ is absorbs via multiplication. Next, let $j_1+I,j_2+I \in J/I$. Then
	\begin{equation*}
		j_1+I+j_2+I = (j_1+j_2)+I
	\end{equation*}
	Since $J$ is an ideal, $j_1+j_2 \in J$. Thus, $J/I$ is closed under addition. Therfore, $J/I$ is an ideal.
	Thus, $J/I$ is an ideal. Conversely, if $K \unlhd R/I$, then the preimage
	\[
	\pi^{-1}(K) = \{ r \in R : r+I \in K \}
	\]
	is an ideal of $R$ containing $I$. Moreover, these assignments are
	inverse to each other:
	\[
	\pi^{-1}(J/I) = J \quad \text{and} \quad \pi(\pi^{-1}(K)) = K.
	\]
	Hence there is a bijection between ideals of $R$ containing $I$ and
	ideals of $R/I$, given by
	\[
	J \longleftrightarrow J/I.
	\]
\end{proof}

\subsection{The Evaluation Map}